STLC.v done through soundness

STLC.v
@@ -3,11 +3,14 @@ Require Import partial_map.
 
 Module STLC.
 
+Hint Resolve beq_id_eq beq_id_false_not_eq.
+  
 (* types *)
 Inductive type : Type :=
 | TBool : type
 | TArrow : type -> type -> type.
 
+Hint Constructors type.
 
 (* terms *)
 Inductive term : Type :=
@@ -20,70 +23,227 @@ Inductive term : Type :=
 
 Notation "\ x : t1 . y" := (TLambda x t1 y) (at level 50).
 
+Tactic Notation "term_cases" tactic(first) ident(c) :=
+  first;
+  [ Case_aux c "TVar"    | Case_aux c "TApp"
+  | Case_aux c "TLambda" | Case_aux c "TTrue"
+  | Case_aux c "TFalse"  | Case_aux c "TIf" ].
+
+Hint Constructors term.
 
 Inductive value : term -> Prop :=
 | v_abs : forall x T t, value (TLambda x T t)
 | v_true : value TTrue
 | v_false : value TFalse.
 
+Hint Constructors value.
 
 Fixpoint subst (x : id) (s : term) (t : term) : term :=
   match t with
-  | TVar x' =>
-     if beq_id x x' then s else t
-  | TLambda x' T t1 =>
-     TLambda x' T (if beq_id x x' then t1 else (subst x s t1))
-  | TApp lambda arg =>
-     TApp (subst x s lambda) (subst x s arg)
-  | TTrue => TTrue
-  | TFalse => TFalse
-  | TIf c t e => TIf (subst x s c) (subst x s t) (subst x s e)
+    | TVar x' =>
+      if beq_id x x' then s else t
+    | TLambda x' T t1 =>
+      TLambda x' T (if beq_id x x' then t1 else (subst x s t1))
+    | TApp lambda arg =>
+      TApp (subst x s lambda) (subst x s arg)
+    | TTrue => TTrue
+    | TFalse => TFalse
+    | TIf c t e => TIf (subst x s c) (subst x s t) (subst x s e)
   end.
 
 Notation "'[' x ':=' s ']' t" := (subst x s t) (at level 20).
 
-
-
 Reserved Notation "t1 '=>' t2" (at level 40).
 Inductive step : term -> term -> Prop :=
 | ST_AppLambda : forall x T t12 v2,
-                 value v2 -> (TApp (TLambda x T t12) v2) => [x := v2]t12
+                   value v2 -> (TApp (TLambda x T t12) v2) => [x := v2]t12
 | ST_App1 : forall t1 t1' t2, t1 => t1' -> TApp t1 t2 => TApp t1' t2
 | ST_App2 : forall v1 t2 t2', value v1 -> t2 => t2' -> TApp v1 t2 => TApp v1 t2'
 | ST_IfTrue : forall t1 t2, TIf TTrue t1 t2 => t1
 | ST_IfFalse : forall t1 t2, TIf TFalse t1 t2 => t2
 | ST_If : forall t1 t1' t2 t3, t1 => t1' -> TIf t1 t2 t3 => TIf t1' t2 t3
-where "t1 '=>' t2" := (step t1 t2).
+    where "t1 '=>' t2" := (step t1 t2).
 
 Tactic Notation "step_cases" tactic(first) ident(c) :=
   first;
   [ Case_aux c "ST_AppLambda" | Case_aux c "ST_App1"
-  | Case_aux c "ST_App2"      | Case_aux c "ST_IfTrue"
-  | Case_aux c "ST_IfFalse"   | Case_aux c "ST_If" ].
+    | Case_aux c "ST_App2"      | Case_aux c "ST_IfTrue"
+    | Case_aux c "ST_IfFalse"   | Case_aux c "ST_If" ].
+
+Hint Constructors step.
 
 Notation multistep := (multi step).
 Notation "t1 '=>*' t2" := (multistep t1 t2) (at level 40).
-
-
-
 
 Definition context := partial_map type.
 
 Inductive has_type : context -> term -> type -> Prop :=
 | T_Var : forall G x T,
-          G x = Some T -> has_type G (TVar x) T
+            G x = Some T -> has_type G (TVar x) T
 | T_Lambda : forall G x T11 T12 t12,
-             has_type (extend G x T11) t12 T12 ->
-             has_type G (TLambda x T11 t12) (TArrow T11 T12)
+               has_type (extend G x T11) t12 T12 ->
+               has_type G (TLambda x T11 t12) (TArrow T11 T12)
 | T_App : forall T11 T12 G t1 t2,
-          has_type G t1 (TArrow T11 T12) ->
-          has_type G t2 T11 ->
-          has_type G (TApp t1 t2) T12
+            has_type G t1 (TArrow T11 T12) ->
+            has_type G t2 T11 ->
+            has_type G (TApp t1 t2) T12
 | T_True : forall G, has_type G TTrue TBool
 | T_False : forall G, has_type G TFalse TBool
 | T_If : forall t1 t2 t3 T G,
-         has_type G t1 TBool ->
-         has_type G t2 T ->
-         has_type G t3 T ->
-         has_type G (TIf t1 t2 t3) T.
+           has_type G t1 TBool ->
+           has_type G t2 T ->
+           has_type G t3 T ->
+           has_type G (TIf t1 t2 t3) T.
 
+Tactic Notation "has_type_cases" tactic(first) ident(c) :=
+  first;
+  [ Case_aux c "T_Var"   | Case_aux c "T_Lambda"
+  | Case_aux c "T_App"   | Case_aux c "T_True"
+  | Case_aux c "T_False" | Case_aux c "T_If" ].
+
+Hint Constructors has_type.
+Hint Unfold beq_nat beq_id extend.
+
+Theorem progress : forall t T, 
+     has_type empty t T ->
+     value t \/ exists t', t => t'.
+Proof with eauto.
+  intros t T Ht.
+  remember empty as gamma.
+  has_type_cases (induction Ht) Case; subst... 
+  Case "T_Var". inversion H.
+  Case "T_App". right. destruct IHHt1...
+    SCase "t1 is a value". destruct IHHt2...
+      SSCase "t2 is a value".
+        inversion H; subst; try solve by inversion.
+        exists ([x := t2] t). constructor...
+      SSCase "t2 steps". inversion H0. exists (TApp t1 x). constructor...
+    SCase "t1 steps". inversion H. exists (TApp x t2). constructor...
+  Case "T_If". right. destruct IHHt1...
+    SCase "t1 is a value". inversion H; subst; try solve by inversion.
+      SSCase "if true". exists t2. constructor.
+      SSCase "if false". exists t3. constructor.
+    inversion H. exists (TIf x t2 t3). constructor...
+Qed.
+
+Inductive appears_free_in : id -> term -> Prop :=
+| AFI_Var : forall x,
+              appears_free_in x (TVar x)
+| AFI_App1 : forall x t1 t2,
+               appears_free_in x t1 -> appears_free_in x (TApp t1 t2)
+| AFI_App2 : forall x t1 t2,
+               appears_free_in x t2 -> appears_free_in x (TApp t1 t2)
+| AFI_Lambda : forall x y T11 t12,
+                 y <> x ->
+                 appears_free_in x t12 ->
+                 appears_free_in x (TLambda y T11 t12)
+| AFI_If1 : forall x t1 t2 t3,
+              appears_free_in x t1 ->
+              appears_free_in x (TIf t1 t2 t3)
+| AFI_If2 : forall x t1 t2 t3,
+              appears_free_in x t2 ->
+              appears_free_in x (TIf t1 t2 t3)
+| AFI_If3 : forall x t1 t2 t3,
+              appears_free_in x t3 ->
+              appears_free_in x (TIf t1 t2 t3).
+
+Tactic Notation "afi_cases" tactic(first) ident(c) :=
+  first;
+  [ Case_aux c "AFI_Var"  | Case_aux c "AFI_App1"
+  | Case_aux c "AFI_App2" | Case_aux c "AFI_Lambda"
+  | Case_aux c "AFI_If1"  | Case_aux c "AFI_If2"
+  | Case_aux c "AFI_If3" ].
+
+Hint Constructors appears_free_in.
+
+Definition closed (t:term) := forall x, ~ appears_free_in x t.
+
+Lemma free_in_context : forall x t T gamma,
+                          appears_free_in x t ->
+                          has_type gamma t T ->
+                          exists T', gamma x = Some T'.
+Proof.
+  intros x t T gamma H H0. generalize dependent gamma.
+  generalize dependent T.
+  afi_cases (induction H) Case; intros; try solve [inversion H0; eauto].
+    Case "AFI_Lambda". inversion H1. subst. apply IHappears_free_in in H7.
+      apply not_eq_beq_id_false in H. rewrite extend_neq in H7; assumption.
+Qed.
+
+Lemma context_invariance : forall gamma gamma' t T,
+                             has_type gamma t T ->
+                             (forall x, appears_free_in x t -> gamma x = gamma' x) ->
+                             has_type gamma' t T.
+Proof with eauto.
+  intros.
+  generalize dependent gamma'.
+  has_type_cases (induction H) Case; intros; auto.
+  Case "T_Var". apply T_Var. rewrite <- H0...
+  Case "T_Lambda". apply T_Lambda. apply IHhas_type. intros x0 Hafi.
+    unfold extend. remember (beq_id x x0). destruct b...
+  Case "T_App".
+    eapply T_App...
+Qed.
+
+Lemma substitution_preserves_typing : forall gamma x U t t' T,
+                                        has_type (extend gamma x U) t T ->
+                                        has_type empty t' U ->
+                                        has_type gamma ([x:=t']t) T.
+Proof with eauto.
+  intros gamma x U t t' T Ht Ht'.
+  generalize dependent gamma. generalize dependent T.
+  term_cases (induction t) Case; intros T gamma H; inversion H; subst; simpl...
+  Case "TVar". rename i into y. remember (beq_id x y) as e. destruct e.
+    SCase "x=y". apply beq_id_eq in Heqe. subst. rewrite extend_eq in H2.
+      inversion H2. subst. eapply context_invariance... intros x Hcontra.
+      destruct (free_in_context _ _ T empty Hcontra)... inversion H0.
+    SCase "x<>y". constructor. rewrite extend_neq in H2...
+  Case "TLambda". rename i into y. apply T_Lambda.
+    remember (beq_id x y) as e. destruct e.
+    SCase "x=y". eapply context_invariance... apply beq_id_eq in Heqe. subst.
+      intros x Hafi. unfold extend. remember (beq_id y x) as e. destruct e...
+    SCase "x<>y".
+      apply IHt. eapply context_invariance... intros z Hafi. unfold extend.
+      remember (beq_id y z) as e0. destruct e0...
+      apply beq_id_eq in Heqe0. subst.
+      rewrite <- Heqe...
+Qed.
+
+Theorem preservation : forall t t' T,
+                         has_type empty t T ->
+                         t => t' ->
+                         has_type empty t' T.
+Proof with eauto.
+  remember empty as gamma.
+  intros t t' T HT. generalize dependent t'.
+  has_type_cases (induction HT) Case;
+    intros t' HE; subst;  
+       try solve [inversion HE; subst; auto].
+  Case "T_App".
+    inversion HE; subst...
+    (* Most of the cases are immediate by induction, 
+       and eauto takes care of them *)
+    SCase "ST_AppAbs".
+      apply substitution_preserves_typing with T11...
+      inversion HT1...
+Qed.
+
+Definition normal_form {X:Type} (R:relation X) (t:X) : Prop :=
+  ~ exists t', R t t'.
+  
+Definition stuck (t : term) : Prop :=
+  (normal_form step) t /\ ~ value t.
+
+Corollary soundness : forall t t' T,
+  has_type empty t T -> 
+  t =>* t' ->
+  ~(stuck t').
+Proof with auto.
+  intros t t' T Hhas_type Hmulti. unfold stuck.
+  intros [Hnf Hnot_val]. unfold normal_form in Hnf.
+  multi_cases (induction Hmulti) Case.
+  Case "multi_refl".
+    apply progress in Hhas_type. inversion Hhas_type...
+  Case "multi_step".
+    apply preservation with (t' := y) in Hhas_type...
+Qed.
